proofs check, verification succeeds

src/schnorr_protocol.h
@@ -3,7 +3,6 @@
 typedef uint64_t bignum[NLIMBS];
 
 extern void __commitment(
-                         // TODO: or: bignum commitment_p or bignum *commitment_p
    uint64_t *commitment_p,      /* NLIMBS output  */
    uint64_t *random_power_p     /* NLIMBS output  */
 );
@@ -11,7 +10,6 @@ extern void __commitment(
 extern void __response(
    uint64_t *random_power_p,    /* NLIMBS input */
    uint64_t *challenge_p,       /* NLIMBS input */
-   uint64_t *witness_p,         /* NLIMBS input (parameter) */
    uint64_t *response_p         /* NLIMBS output */
 );
 
@@ -20,7 +18,6 @@ extern void __challenge(
 );
 
 extern void __verify(
-   uint64_t *statement_p,      /* NLIMBS input (parameter) */
    uint64_t *commitment_p,     /* NLIMBS input */
    uint64_t *challenge_p,      /* NLIMBS input */
    uint64_t *response_p,       /* NLIMBS input */
